% !TEX root = /Users/solveig/Documents/PhD/fourspheremodel/doc/sphere4_to_sphere3.tex
\documentclass{article}
\usepackage[utf8]{inputenc}
\usepackage[T1]{fontenc}
\usepackage[english]{babel}
\usepackage{amsmath}
\usepackage{graphicx}
\usepackage{caption}
\usepackage{subcaption}
\usepackage[margin=1.4in]{geometry}
\usepackage{float}
\usepackage{array}
\usepackage{rotating}
\usepackage[labelfont={bf,up}, font={small}]{caption}
\usepackage{sidecap}
\sidecaptionvpos{figure}{c}
\usepackage[colorinlistoftodos]{todonotes}
\usepackage{adjustbox}
\usepackage{placeins}
\usepackage{xcolor}

\title{Reduction from 4-sphere model to 3-sphere model as $r_4 \to r_3$ and $\sigma_4 \to \sigma_3$}

\author{Solveig NÃ¦ss \\ \textit{solvenae@ifi.uio.no} }

\date{\today}
\begin{document}
\maketitle
As an extra validation of the corrected formulas for the four-sphere model for EEG signals, we here present a limiting case. The four-sphere model should reduce to the three-sphere model when the radii and electrical conductivities are equal for sphere three and four. 
\begin{align*}
\Phi^4(r, \theta) &= \Phi^3(r, \theta) \quad \forall~~ r_4 \to r_3
\end{align*}

\begin{equation}\label{eq:phi_sphere_3}
\Phi^3(r) = \frac{p}{4 \pi \sigma_1 r_z^2}\sum_{n = 1}^{\infty} \big[ A_3^s \big(\frac{r}{r_3}\big)^n + B_n^3\big(\frac{r_3}{r}\big)^{n+1}\big] n P_n(\cos{\theta})
\end{equation}
\begin{equation}\label{eq:phi_sphere_4}
\Phi^4(r) = \frac{p}{4 \pi \sigma_1 r_z^2}\sum_{n = 1}^{\infty} \big[ A_4^s \big(\frac{r}{r_4}\big)^n + B_n^4\big(\frac{r_4}{r}\big)^{n+1}\big] n P_n(\cos{\theta})
\end{equation}
Inserting $r_3 = r_4$ into the expression for $\Phi^4$, we can see that the requirement is fulfilled when $A_n^4 = A_n^3$ and $B_n^4 = B_n^3$.
\\\\
As $r_4 \to r_3$ and $\sigma_4 \to \sigma_3$, we get the following expressions for $A_n^4$
\begin{align*}
A_n^4 &= \frac{n+1}{n} \frac{A_n^3 + B_n^3}{\frac{n+1}{n} r_{34}^n + r_{43}^{n+1}} \\
&= (A_n^3 + B_n^3) \frac{\frac{n+1}{n}}{\frac{n+1}{n} + 1},
\end{align*}
and $B_n^3$
\begin{align*}
B_n^3 &= V_n A_n^3 \\
&= A_n^3 \frac{ \frac{n}{n+1} \sigma_{34} - \frac{r_{34}^n - r_{43}^{n+1}}{\frac{n+1}{n} r_{34}^n + r_{43}^{n+1}}}{\sigma_{34} + \frac{r_{34}^n - r_{43}^{n+1}}{\frac{n+1}{n} r_{34}^n + r_{43}^{n+1}}} \\
&= \frac{n}{n+1}A_n^3.
\end{align*}
From here we can combine the two relations above, such that
\begin{align*}
A_n^4 &= A_n^3 \frac{\frac{n+1}{n}(1 + \frac{n}{n+1})}{\frac{n+1}{n} + 1} = A_n^3,
\end{align*}
and find that $A_n^4 = A_n^3$ for $r_4=r_3$ and $\sigma_4 = \sigma_3$.
\\\\
Next we insert this into the expression for $B_n^4$, and make use of the relation $A_n^3 = \frac{n+1}{n}B_n^3$ from above
\begin{align*}
B_n^4 &= \frac{n}{n+1}A_n^4 \\
&= \frac{n}{n+1}A_n^3 \\
&= \frac{n}{n+1} \frac{n+1}{n} B_n^3 \\
&= B_n^3,
\end{align*}
and obtain that $B_n^4 = B_n^3$ for $r_4=r_3$ and $\sigma_4 = \sigma_3$.
\end{document}